src/CSL/RefinementIdempotenceFunModule.v
@@ -1,0 +1,262 @@
+(* We specialize some of the idempotence module construction results to the special
+   case when compilation is defined as a per-op translation. *)
+
+From Transitions Require Import Relations Rewriting.
+
+Require Import Spec.Proc.
+Require Import Spec.ProcTheorems.
+Require Import Spec.Layer.
+Require Export CSL.WeakestPre CSL.Refinement CSL.Adequacy  CSL.RefinementAdequacy CSL.ThreadReg.
+Require CSL.RefinementIdempotenceModule.
+From iris.algebra Require Import auth frac agree gmap list.
+From iris.base_logic.lib Require Import invariants.
+From iris.proofmode Require Import tactics.
+Unset Implicit Arguments.
+
+Import RelationNotations.
+From Transitions Require Import Relations.
+
+Module Type refinement_type.
+  Context (OpC OpT: Type → Type).
+  Context (Λc: Layer OpC) (Λa: Layer OpT).
+  Context (impl: LayerImpl OpC OpT).
+  Context (Σ: gFunctors).
+  Context (exmachG : gFunctors → Type).
+  Existing Class exmachG.
+  Notation compile_op := (compile_op impl).
+  Notation compile_rec := (compile_rec impl).
+  Notation compile_seq := (compile_seq impl).
+  Notation compile := (compile impl).
+  Notation recover := (recover impl).
+  Notation compile_proc_seq := (compile_proc_seq impl).
+  Context `{CFG: cfgPreG OpT Λa Σ}.
+  Context `{INV: Adequacy.invPreG Σ}.
+  Context `{REG: inG Σ (csumR countingR (authR (optionUR (exclR unitC))))}.
+  Context {Hinstance: ∀ Σ, exmachG Σ → irisG OpC Λc Σ}.
+  Context {Hinstance_reg: ∀ Σ, exmachG Σ → tregG Σ}.
+  Context (crash_inner: forall {_ : @cfgG OpT Λa Σ} {_: exmachG Σ}, iProp Σ).
+  Context (exec_inner: forall {_ : @cfgG OpT Λa Σ} {_: exmachG Σ}, iProp Σ).
+  Context (crash_param: forall (_ : @cfgG OpT Λa Σ) (_ : exmachG Σ), Type).
+  Context (crash_inv: forall {H1 : @cfgG OpT Λa Σ} {H2 : exmachG Σ},
+              @crash_param _ H2 → iProp Σ).
+  Context (crash_starter: forall {H1 : @cfgG OpT Λa Σ} {H2 : exmachG Σ},
+              @crash_param _ H2 → iProp Σ).
+  Context (exec_inv: forall {_ : @cfgG OpT Λa Σ} {_ : exmachG Σ}, iProp Σ).
+
+  Context (E: coPset).
+  (* TODO: we should get rid of rec_seq if we're not exploiting vertical comp anymore *)
+  Context (recv: proc OpC unit).
+
+  (* TODO: probably should say that this has to be given using Tej's record setter stuff *)
+  Context (set_inv_reg: exmachG Σ → invG Σ → tregG Σ → exmachG Σ).
+  Context (init_absr: Λa.(OpState) → Λc.(OpState) → Prop).
+
+End refinement_type.
+
+Module refinement_definitions (RT: refinement_type).
+
+  Import RT.
+  Existing Instances Hinstance Hinstance_reg.
+
+  Definition set_reg (Hex: exmachG Σ) (tR: tregG Σ) :=
+    set_inv_reg Hex _ tR.
+  Definition set_inv (Hex: exmachG Σ) (Hinv: invG Σ) :=
+    set_inv_reg Hex Hinv _.
+
+  Definition post_crash {Hex: exmachG Σ} (P: ∀ {_: exmachG Σ}, iProp Σ) : iProp Σ :=
+    (∀ Hreg', |={E}=> ∀ n σ σ' (Hcrash: Λc.(crash_step) σ (Val σ' tt)),
+        state_interp (n, σ) ∗ @thread_count_interp _ Hreg' 1 ==∗
+                     ∃ Hex', let _ := set_reg Hex' Hreg' in
+                             state_interp (1, σ') ∗ P)%I.
+
+  Definition post_finish {Hex: exmachG Σ} (P: ∀ {_: exmachG Σ}, iProp Σ) : iProp Σ :=
+    (∀ n σ σ' (Hcrash: Λc.(finish_step) σ (Val σ' tt)) Hinv' Hreg',
+        state_interp (n, σ) ∗ @thread_count_interp _ Hreg' 1 ==∗
+                     ∃ Hex', let _ := set_inv_reg Hex' Hinv' Hreg' in
+                             state_interp (1, σ') ∗ P)%I.
+
+  Definition post_recv {Hex: exmachG Σ} (P: ∀ {_: exmachG Σ}, iProp Σ) : iProp Σ :=
+    (∀ n σ Hinv' Hreg',
+        state_interp (n, σ) ∗ @thread_count_interp _ Hreg' 1 ==∗
+                     ∃ Hex', let _ := set_inv_reg Hex' Hinv' Hreg' in
+                             state_interp (1, σ) ∗ P)%I.
+
+  Definition recv_triple_type :=
+    ∀ H1 H2 param,
+      (@crash_inv H1 H2 param) ∗ Registered ∗ (@crash_starter H1 H2 param) ⊢
+              WP recv @ NotStuck; ⊤
+                 {{ v, |={⊤,E}=> ∃ σ2a σ2a', source_state σ2a
+                       ∗ ⌜Λa.(crash_step) σ2a (Val σ2a' tt)⌝ ∗
+                       ∀ `{Hcfg': cfgG OpT Λa Σ},
+                         post_recv (λ H, source_ctx ∗ source_state σ2a' ==∗ |={⊤}=> exec_inner Hcfg' H
+                                    )}}.
+
+  Definition init_exec_inner_type :=
+    ∀ σ1a σ1c, init_absr σ1a σ1c →
+      (∀ `{Hinv: invG Σ} Hreg `{Hcfg: cfgG OpT Λa Σ},
+          |={⊤}=> ∃ (Hex': exmachG Σ),
+         (source_ctx ∗ source_state σ1a ∗ @thread_count_interp _ Hreg 1)
+           ={⊤}=∗ let _ := set_inv_reg Hex' Hinv Hreg in
+                  exec_inner Hcfg _ ∗ state_interp (1, σ1c))%I.
+
+  Definition exec_inv_preserve_crash_type :=
+      (∀ `(Hex: exmachG Σ) `(Hcfg: cfgG OpT Λa Σ),
+          exec_inv Hcfg Hex ={⊤, E}=∗ post_crash (λ H, |==> crash_inner Hcfg H)).
+
+  Definition crash_inv_preserve_crash_type :=
+      (∀ `(Hex: exmachG Σ) `(Hcfg: cfgG OpT Λa Σ) param,
+          crash_inv Hcfg Hex param ={⊤, E}=∗ post_crash (λ H, |==> crash_inner Hcfg H)).
+
+  Definition state_interp_no_inv_type :=
+      (∀ `(Hex: exmachG Σ) Hinv σ,
+           state_interp σ -∗ let _ := set_inv Hex Hinv in state_interp σ).
+
+  Definition crash_inner_inv_type :=
+      (∀ `(Hex: exmachG Σ) `(Hcfg: cfgG OpT Λa Σ),
+          (∃ Hinv, crash_inner Hcfg (set_inv Hex Hinv)) ∗ source_ctx ={⊤}=∗
+          ∃ param, crash_inv Hcfg Hex param ∗ crash_starter Hcfg Hex param).
+
+  Definition exec_inner_inv_type :=
+      (∀ (Hex: exmachG Σ) `(Hcfg: cfgG OpT Λa Σ),
+          (∃ Hinv, exec_inner Hcfg (set_inv Hex Hinv))
+          ∗ source_ctx ={⊤}=∗ exec_inv Hcfg Hex).
+
+  Definition exec_inv_preserve_finish_type :=
+      (∀ `(Hex: exmachG Σ) `(Hcfg: cfgG OpT Λa Σ),
+          AllDone -∗ exec_inv Hcfg Hex ={⊤, E}=∗ ∃ (σ2a σ2a' : Λa.(OpState)), source_state σ2a
+          ∗ ⌜Λa.(finish_step) σ2a (Val σ2a' tt)⌝ ∗
+          ∀ `{Hcfg': cfgG OpT Λa Σ},
+          post_finish (λ H, source_ctx ∗ source_state σ2a' ==∗ |={⊤}=> exec_inner Hcfg' H)).
+
+End refinement_definitions.
+
+Module Type refinement_obligations (RT: refinement_type).
+
+  Import RT.
+  Module RD := refinement_definitions RT.
+  Import RD.
+
+  Context (einv_persist: forall {H1 : @cfgG OpT Λa Σ} {H2 : _},
+              Persistent (exec_inv H1 H2)).
+  Context (cinv_persist: forall {H1 : @cfgG OpT Λa Σ} {H2 : _}
+            {P: crash_param _ _}, Persistent (crash_inv H1 H2 P)).
+  Context (nameIncl: nclose sourceN ⊆ E).
+  Context (recsingle: recover = rec_singleton recv).
+  Context (exec_inv_source_ctx: ∀ {H1 H2}, exec_inv H1 H2 ⊢ source_ctx).
+
+
+  Context (set_inv_reg_spec0:
+             ∀ Hex, (set_inv_reg Hex (Hinstance Σ Hex).(@iris_invG OpC (State Λc) Σ)
+                                                         (Hinstance_reg Σ Hex) = Hex)).
+  Context (set_inv_reg_spec1:
+             ∀ Hex Hinv Hreg, @iris_invG _ _ _ (Hinstance _ (set_inv_reg Hex Hinv Hreg)) = Hinv).
+  Context (set_inv_reg_spec2:
+             ∀ Hex Hinv Hreg, Hinstance_reg _ (set_inv_reg Hex Hinv Hreg) = Hreg).
+  Context (set_inv_reg_spec3:
+             ∀ Hex Hinv Hinv' Hreg Hreg', set_inv_reg (set_inv_reg Hex Hinv' Hreg') Hinv Hreg =
+                              (set_inv_reg Hex Hinv Hreg)).
+
+  Context (register_spec: ∀ {H: exmachG Σ}, ∃ (Interp: OpState Λc → iProp Σ),
+                (∀ n σ, @state_interp _ _ _ (Hinstance _ H) (n, σ)
+                                     -∗ thread_count_interp n ∗ Interp σ) ∧
+                ∀ n σ, thread_count_interp n ∗ Interp σ -∗ state_interp (n, σ)).
+
+  Context (refinement_op_triples:
+             forall {H1 H2 T1 T2} j K `{LanguageCtx OpT T1 T2 Λa K} (op: OpT T1),
+               j ⤇ K (Call op) ∗ Registered ∗ (@exec_inv H1 H2) ⊢
+                 WP compile (Call op) {{ v, j ⤇ K (Ret v) ∗ Registered  }}).
+
+  (* State interpretations should not contain invariants *)
+
+  Context (state_interp_no_inv: state_interp_no_inv_type).
+
+  Context (recv_triple: recv_triple_type).
+  Context (init_exec_inner: init_exec_inner_type).
+  Context (exec_inv_preserve_crash: exec_inv_preserve_crash_type).
+  Context (crash_inv_preserve_crash: crash_inv_preserve_crash_type).
+  Context (exec_inner_inv: exec_inner_inv_type).
+  Context (crash_inner_inv: crash_inner_inv_type).
+  Context (exec_inv_preserve_finish : exec_inv_preserve_finish_type).
+End refinement_obligations.
+
+
+Module refinement (RT: refinement_type) (RO: refinement_obligations RT).
+  Import RT RO.
+  Existing Instances Hinstance Hinstance_reg einv_persist cinv_persist.
+
+  Import Reg_wp.
+
+  Module RT' <: RefinementIdempotenceModule.refinement_type.
+    Definition OpC := OpC.
+    Definition Λc := Λc.
+    Definition OpT := OpT.
+    Definition Λa := Λa.
+    Definition impl := LayerImpl_to_LayerImplRel impl.
+    Definition exmachG := exmachG.
+    Definition Σ := Σ.
+    Definition CFG := CFG.
+    Definition INV := INV.
+    Definition REG := REG.
+    Definition Hinstance := Hinstance.
+    Definition Hinstance_reg := Hinstance_reg.
+    Definition set_inv_reg := set_inv_reg.
+
+    Definition crash_inner := crash_inner.
+    Definition exec_inner := exec_inner.
+    Definition crash_inv := crash_inv.
+    Definition crash_param := crash_param.
+    Definition crash_starter := crash_starter.
+    Definition exec_inv := exec_inv.
+    Definition E := E.
+    Definition recv := recv.
+    Definition init_absr := init_absr.
+  End RT'.
+
+  Module RD := RefinementIdempotenceModule.refinement_definitions RT'.
+  Module RO' <: RefinementIdempotenceModule.refinement_obligations RT'.
+    Module RD := RD.
+    Definition nameIncl := RO.nameIncl.
+    Definition einv_persist := RO.einv_persist.
+    Definition cinv_persist := RO.cinv_persist.
+    Existing Instances einv_persist cinv_persist.
+    Definition recsingle := RO.recsingle.
+    Definition refinement_op_triples := RO.refinement_op_triples.
+    Definition exec_inv_source_ctx := RO.exec_inv_source_ctx.
+    Definition set_inv_reg_spec0 := RO.set_inv_reg_spec0.
+    Definition set_inv_reg_spec1 := RO.set_inv_reg_spec1.
+    Definition set_inv_reg_spec2 := RO.set_inv_reg_spec2.
+    Definition set_inv_reg_spec3 := RO.set_inv_reg_spec3.
+    Definition register_spec := RO.register_spec.
+    Definition recv_triple := RO.recv_triple.
+    Definition init_exec_inner := RO.init_exec_inner.
+    Definition exec_inv_preserve_crash := RO.exec_inv_preserve_crash.
+    Definition crash_inv_preserve_crash := RO.crash_inv_preserve_crash.
+    Definition state_interp_no_inv := RO.state_interp_no_inv.
+    Definition crash_inner_inv := RO.crash_inner_inv.
+    Definition exec_inner_inv := RO.exec_inner_inv.
+    Definition exec_inv_preserve_finish := RO.exec_inv_preserve_finish.
+
+    Lemma refinement_base_triples : RD.refinement_base_triples_type.
+      intros ???? j K ? p p' (op&Heq1&Heq2). subst. iApply refinement_op_triples.
+    Qed.
+  End RO'.
+
+  Module R := RefinementIdempotenceModule.refinement RT' RO'.
+
+  Lemma crash_refinement_seq {T} σ1c σ1a (es: proc_seq OpT T) :
+    init_absr σ1a σ1c →
+    wf_client_seq es →
+    ¬ proc_exec_seq Λa es (rec_singleton (Ret ())) (1, σ1a) Err →
+    ∀ σ2c res, proc_exec_seq Λc (compile_proc_seq es) (rec_singleton recv) (1, σ1c) (Val σ2c res) →
+    ∃ σ2a, proc_exec_seq Λa es (rec_singleton (Ret tt)) (1, σ1a) (Val σ2a res).
+  Proof.
+    intros. eapply R.crash_refinement_seq; eauto.
+    clear.
+    induction es; econstructor; eauto.
+    clear. econstructor. induction p; eauto; try (repeat econstructor; done).
+    * eapply cr_bind; eauto.
+    * eapply cr_loop; eauto.
+    * eapply cr_spawn; eauto.
+  Qed.
+
+End refinement.
